iris/UnionLinks.v
@@ -58,7 +58,7 @@ From stdpp Require Import list.
 Local Open Scope list_scope.
 
 Local Notation U := ulmG.
-Local Notation UB := (ulm_byte_laws adm_u_g adm_s_off).
+Local Notation UB := (ulm_byte_laws adm_u_g adm_s_on).
 
 Section union_links.
   Context {Σ : gFunctors}.
