iris/UnionReadInstAt.v
@@ -82,7 +82,7 @@ Proof using.
   rewrite ins_app ins_in in Hseg.
   assert (Hin' : b ∈ ins s0 ++ [b]).
   { apply elem_of_app. right. by apply elem_of_list_singleton. }
-  pose proof (lm_disc_input_byte_val U (ulm_byte_laws adm_u_g adm_s_off) (ins s0 ++ [b]) b
+  pose proof (lm_disc_input_byte_val U (ulm_byte_laws adm_u_g adm_s_on) (ins s0 ++ [b]) b
                 Hseg Hin') as Hv.
   lia.
 Qed.
